Move points-to definitions into resources

src/high/resources.v
@@ -2,11 +2,13 @@
 high-level logic. *)
 From iris.base_logic.lib Require Import own ghost_map.
 From iris.algebra Require Import gset gmap excl auth.
+From iris.proofmode Require Import reduction monpred tactics.
+From iris_named_props Require Import named_props.
 
 From self Require Import extra.
 From self.lang Require Import lang.
 From self.base Require Import primitive_laws.
-From self.high Require Import dprop.
+From self.high Require Import dprop lifted_modalities.
 
 (* Resource algebra used to represent agreement on which predicates are
 associated with which locations. *)
@@ -58,3 +60,532 @@ Class AbstractState T := {
 
 Instance abstract_state_sqsubseteq `{AbstractState T} : SqSubsetEq T :=
   abs_state_relation.
+
+Global Instance discretizable_ghost_map_elem `{ghost_mapG Σ K V} ℓ γ v :
+  own_discrete.Discretizable (ℓ ↪[γ] v).
+Proof. rewrite ghost_map_elem_eq /ghost_map_elem_def. apply _. Qed.
+
+(** We define a few things about the resource algebra that that we use to encode
+abstract histories. *)
+Section abs_history_lemmas.
+  Context `{hG : nvmG Σ}.
+  Context `{Countable ST}.
+
+  Implicit Types (abs_hist : gmap time ST) (ℓ : loc).
+  Implicit Types (abs_hists : gmap loc (gmap time positive)).
+
+  Definition abs_hist_to_ra abs_hist : encoded_abs_historyR :=
+    (to_agree ∘ encode) <$> abs_hist.
+
+  Definition own_full_history_gname γ1 γ2 abs_hists : iProp Σ :=
+    ghost_map_auth γ1 1 abs_hists ∗
+    own γ2
+        (● ((λ m : gmap _ _, to_agree <$> m) <$> abs_hists) : know_abs_historiesR).
+
+  Definition own_full_history abs_hists : iProp Σ :=
+    own_full_history_gname abs_history_name know_abs_history_name abs_hists.
+
+  Definition know_full_history_loc ℓ abs_hist : iProp Σ :=
+    ℓ ↪[ abs_history_name ] (encode <$> abs_hist).
+
+  Definition know_full_encoded_history_loc ℓ (abs_hist : gmap time positive) : iProp Σ :=
+    ℓ ↪[ abs_history_name ] abs_hist.
+
+  Definition know_frag_history_loc ℓ (abs_hist : abs_history ST) : iProp Σ :=
+    ∃ enc,
+      ⌜(decode <$> enc = Some <$> abs_hist)⌝ ∗
+      own know_abs_history_name (◯ {[ ℓ := to_agree <$> enc ]}).
+
+  Lemma own_full_history_gname_alloc h :
+    ⊢ |==> ∃ γ1 γ2,
+        own_full_history_gname γ1 γ2 h ∗
+        own γ2 (◯ ((λ m : gmap _ _, to_agree <$> m) <$> h) : know_abs_historiesR) ∗
+        [∗ map] k↦v ∈ h, k ↪[γ1] v.
+  Proof.
+    iMod (ghost_map_alloc h) as (new_abs_history_name) "[A B]".
+    iExists _. iFrame "A B".
+    setoid_rewrite <- own_op.
+    iMod (own_alloc _) as "$".
+    { apply auth_both_valid_2; last reflexivity.
+      intros k.
+      rewrite lookup_fmap.
+      destruct (h !! k); simpl; last done.
+      apply Some_valid.
+      intros k'.
+      rewrite lookup_fmap.
+      destruct (g !! k'); done. }
+    done.
+  Qed.
+
+  Lemma know_full_equiv ℓ abs_hist :
+    know_full_history_loc ℓ abs_hist ⊣⊢
+      know_full_encoded_history_loc ℓ (encode <$> abs_hist).
+  Proof. done. Qed.
+
+  Lemma abs_hist_to_ra_inj hist hist' :
+    abs_hist_to_ra hist' ≡ abs_hist_to_ra hist →
+    hist' = hist.
+  Proof.
+    intros eq.
+    apply: map_eq. intros t.
+    pose proof (eq t) as eq'.
+    rewrite !lookup_fmap in eq'.
+    destruct (hist' !! t) as [h|] eqn:leq, (hist !! t) as [h'|] eqn:leq';
+      try inversion eq'; auto.
+    simpl in eq'.
+    apply Some_equiv_inj in eq'.
+    apply to_agree_inj in eq'.
+    apply encode_inj in eq'.
+    rewrite eq'.
+    done.
+  Qed.
+
+  Lemma abs_hist_to_ra_agree hist hist' :
+    to_agree <$> hist' ≡ abs_hist_to_ra hist →
+    hist' = encode <$> hist.
+  Proof.
+    intros eq.
+    apply: map_eq. intros t.
+    pose proof (eq t) as eq'.
+    rewrite !lookup_fmap in eq'.
+    rewrite lookup_fmap.
+    destruct (hist' !! t) as [h|] eqn:leq, (hist !! t) as [h'|] eqn:leq';
+      try inversion eq'; auto.
+    simpl in eq'. simpl.
+    apply Some_equiv_inj in eq'.
+    apply to_agree_inj in eq'.
+    f_equiv.
+    apply eq'.
+  Qed.
+
+  (** If you know the full history for a location and own the "all-knowing"
+  resource, then those two will agree. *)
+  Lemma own_full_history_agree ℓ hist hists :
+    own_full_history hists -∗
+    know_full_history_loc ℓ hist -∗
+    ⌜hists !! ℓ = Some (encode <$> hist)⌝.
+  Proof.
+    iIntros "[A _] B".
+    iApply (ghost_map_lookup with "[$] [$]").
+  Qed.
+
+  Lemma own_frag_history_agree ℓ (part_hist : gmap time ST) hists :
+    own_full_history hists -∗
+    know_frag_history_loc ℓ part_hist -∗
+    ⌜∃ hist, hists !! ℓ = Some (hist) ∧ (Some <$> part_hist) ⊆ (decode <$> hist)⌝.
+  Proof.
+    rewrite /own_full_history.
+    iIntros "[O A]".
+    iDestruct 1 as (enc) "[%eq K]".
+    iDestruct (own_valid_2 with "A K") as %[incl _]%auth_both_valid_discrete.
+    apply singleton_included_l in incl.
+    destruct incl as [hist' [look incl]].
+    rewrite lookup_fmap in look.
+    destruct (hists !! ℓ) as [hist|]. 2: { inversion look. }
+    simpl in look.
+    iExists hist.
+    iSplit; first done.
+    rewrite <- eq.
+    move: incl.
+    rewrite <- look.
+    rewrite Some_included_total.
+    rewrite -to_agree_fmap.
+    intros incl.
+    iPureIntro.
+    by apply map_fmap_mono.
+  Qed.
+
+  Lemma own_frag_history_agree_singleton ℓ t (s : ST) hists :
+    own_full_history hists -∗
+    know_frag_history_loc ℓ {[ t := s ]} -∗
+    ⌜∃ hist enc,
+      hists !! ℓ = Some hist ∧ hist !! t = Some enc ∧ decode enc = Some s⌝.
+  Proof.
+    iIntros "H1 H2".
+    iDestruct (own_frag_history_agree with "H1 H2") as %[hist [look H1]].
+    iExists hist. iPureIntro.
+    rewrite map_fmap_singleton in H1.
+    rewrite -> map_subseteq_spec in H1.
+    specialize H1 with t (Some s).
+    epose proof (H1 _) as H2.
+    Unshelve. 2: { rewrite lookup_singleton. done. }
+    apply lookup_fmap_Some in H2.
+    destruct H2 as (enc & eq & lookHist).
+    exists enc.
+    repeat split; done.
+  Qed.
+
+  Lemma own_full_history_alloc ℓ t encS (s : ST) hists hist :
+    hists !! ℓ = Some hist →
+    hist !! t = Some encS →
+    decode encS = Some s →
+    own_full_history hists ==∗
+    own_full_history hists ∗ know_frag_history_loc ℓ {[ t := s ]}.
+  Proof.
+    iIntros (look lookHist decEq) "[$ H2]".
+    rewrite /own_full_history /know_frag_history_loc.
+    iMod (own_update with "H2") as "[$ H]".
+    { apply (auth_update_dfrac_alloc _ _ {[ ℓ := {[ t := to_agree encS ]} ]}).
+      apply singleton_included_l.
+      eexists _.
+      rewrite lookup_fmap.
+      rewrite look.
+      simpl.
+      split; first reflexivity.
+      rewrite /abs_hist_to_ra.
+      apply Some_included_total.
+      (* rewrite map_fmap_compose. *)
+      (* rewrite !map_fmap_singleton. *)
+      apply singleton_included_l.
+      eexists _.
+      rewrite lookup_fmap.
+      rewrite lookHist.
+      simpl.
+      split; f_equiv. }
+    iExists {[ t := encS ]}.
+    rewrite !map_fmap_singleton.
+    rewrite decEq.
+    iFrame.
+    done.
+  Qed.
+
+  (* This lemma seems false :'( *)
+  (* Lemma own_frag_history_agree ℓ part_hist hists : *)
+  (*   own_full_history hists -∗ *)
+  (*   know_frag_history_loc ℓ part_hist -∗ *)
+  (*   ⌜∃ hist, hists !! ℓ = Some (encode <$> hist) ∧ part_hist ⊆ hist⌝. *)
+  (* Proof. w w *)
+  (*   iIntros "O K". *)
+  (* Admitted. *)
+
+End abs_history_lemmas.
+
+Section predicates.
+  Context `{!nvmG Σ}.
+
+  Definition predO := positive -d> val -d> optionO (dPropO Σ).
+
+  Definition pred_to_ra (pred : positive → val → option (dProp Σ)) : (@predicateR Σ) :=
+    to_agree ((λ a b, Next (pred a b))).
+
+  Definition preds_to_ra (preds : gmap loc (positive → val → option (dProp Σ)))
+    : gmapUR loc (@predicateR Σ) := pred_to_ra <$> preds.
+
+  Definition know_all_preds preds :=
+      own predicates_name (● (pred_to_ra <$> preds) : predicatesR).
+
+  Definition encode_predicate `{Countable s}
+             (ϕ : s → val → dProp Σ) : positive → val → option (dProp Σ) :=
+    λ encS v, (λ s, ϕ s v) <$> decode encS.
+
+  Definition know_pred `{Countable s}
+      (ℓ : loc) (ϕ : s → val → dProp Σ) : iProp Σ :=
+    own predicates_name (◯ {[ ℓ := pred_to_ra (encode_predicate ϕ) ]} : predicatesR).
+
+  Lemma know_predicates_alloc preds :
+    ⊢ |==> ∃ γ, own γ ((● (pred_to_ra <$> preds)) : predicatesR).
+  Proof.
+    iMod (own_alloc _) as "$"; last done.
+    apply auth_auth_valid.
+    intros ℓ.
+    rewrite lookup_fmap.
+    by case (preds !! ℓ).
+  Qed.
+
+  Lemma know_pred_agree `{Countable s} ℓ (ϕ : s → val → dProp Σ) (preds : gmap loc predO) :
+    know_all_preds preds -∗
+    know_pred ℓ ϕ -∗
+    (∃ (o : predO),
+       ⌜preds !! ℓ = Some o⌝ ∗ (* Some encoded predicate exists. *)
+       ▷ (o ≡ encode_predicate ϕ)).
+  Proof.
+    iIntros "O K".
+    rewrite /know_all_preds /know_pred.
+    iDestruct (own_valid_2 with "O K") as "H".
+    iDestruct (auth_both_validI with "H") as "[tmp val]".
+    iDestruct "tmp" as (c) "#eq".
+    rewrite gmap_equivI.
+    iSpecialize ("eq" $! ℓ).
+    rewrite lookup_fmap.
+    rewrite lookup_op.
+    rewrite lookup_singleton.
+    destruct (preds !! ℓ) as [o|] eqn:eq; rewrite eq /=.
+    2: { simpl. case (c !! ℓ); intros; iDestruct "eq" as %eq'; inversion eq'. }
+    iExists o.
+    iSplit; first done.
+    case (c !! ℓ).
+    - intros ?.
+      rewrite /pred_to_ra.
+      rewrite -Some_op.
+      rewrite !option_equivI.
+      rewrite wsat.agree_equiv_inclI.
+      rewrite !discrete_fun_equivI. iIntros (state).
+      iSpecialize ("eq" $! state).
+      rewrite !discrete_fun_equivI. iIntros (v).
+      iSpecialize ("eq" $! v).
+      rewrite later_equivI_1.
+      iNext.
+      iRewrite "eq".
+      done.
+    - rewrite right_id.
+      simpl.
+      rewrite !option_equivI.
+      rewrite agree_equivI.
+      rewrite !discrete_fun_equivI. iIntros (state).
+      iSpecialize ("eq" $! state).
+      rewrite !discrete_fun_equivI. iIntros (v).
+      iSpecialize ("eq" $! v).
+      rewrite later_equivI_1.
+      done.
+    Qed.
+
+End predicates.
+
+(* (* For each location in the heap we maintain the following "meta data". *)
+(* For every location we want to store: A type/set of abstract events, its full *)
+(* abstract history, the invariant assertion. The abstract history maps *)
+(* timestamps to elements of the abstract events. *) *)
+(* Record loc_info := { *)
+(*   l_state : Type; *)
+(* (*   (* l_val : val; *) *) *)
+(* (*   l_ϕ : l_state → val → dProp Σ; *) *)
+(*   l_abstract_history : gmap nat l_state; *)
+(* (*   (* * Type class instances *) *) *)
+(*   l_sqsubseteq : SqSubsetEq l_state; *)
+(*   l_preorder : PreOrder (⊑@{l_state}); *)
+(*   (* We need countable to squash states into [positive] *) *)
+(*   l_eqdecision : EqDecision l_state; *)
+(*   l_countable : Countable l_state; *)
+(* }. *)
+
+(* Existing Instances l_eqdecision l_countable. *)
+
+(* Definition encode_loc_info {Σ} (l : (@loc_info Σ)):= *)
+(*   ((λ '(m, s), (m, encode s)) <$> (l_abstract_history l), *)
+(*    λ v s, (l_ϕ l $ v) <$> decode s). *)
+
+Definition lift2 {A B C} `{MBind M, MRet M, FMap M} (f : A → B → C) (am : M A) (bm : M B) :=
+  a ← am;
+  b ← bm;
+  mret (f a b).
+
+Definition mapply {A B} `{MBind M, FMap M} (mf : M (A → B)) (a : M A) :=
+  mf ≫= (λ f, f <$> a).
+
+(* This notation does not seem to work for some reason. *)
+(* Notation "<*>" := mapply (at level 61, left associativity). *)
+Notation "mf <*> a" := (mapply mf a) (at level 61, left associativity).
+
+Section preorders.
+  Context `{hG : nvmG Σ}.
+  Context `{Countable A}.
+
+  Definition encode_relation (R : relation2 A) : relation2 positive :=
+    λ (a b : positive), default False (R <$> decode a <*> decode b).
+
+  Lemma encode_relation_iff (R : relation2 A) (a b : A) :
+    R a b ↔ (encode_relation R) (encode a) (encode b).
+  Proof.
+    rewrite /encode_relation.
+    rewrite !decode_encode.
+    reflexivity.
+  Qed.
+
+  Definition own_all_preorders_gname γ (preorders : gmap loc (relation2 positive)) :=
+    own γ (● ((to_agree <$> preorders) : gmapUR _ (agreeR relationO))).
+
+  Definition own_all_preorders (preorders : gmap loc (relation2 positive)) :=
+    own_all_preorders_gname preorders_name preorders.
+
+  Definition own_preorder_loc ℓ (preorder : relation2 A) : iProp Σ :=
+    own preorders_name (◯ ({[ ℓ := to_agree (encode_relation preorder) ]})).
+
+  Global Instance persistent_own_preorder_loc ℓ preorder :
+    Persistent (own_preorder_loc ℓ preorder).
+  Proof. apply _. Qed.
+
+  Lemma own_all_preorders_gname_alloc (preorders : gmap loc (relation2 positive)) :
+    ⊢ |==> ∃ γ, own_all_preorders_gname γ preorders.
+  Proof.
+    iMod (own_alloc _) as "$"; last done.
+    apply auth_auth_valid.
+    intros ℓ.
+    rewrite lookup_fmap.
+    by case (preorders !! ℓ).
+  Qed.
+
+  Lemma orders_lookup ℓ order1 order2 (orders : gmap loc (relation2 positive)) :
+    orders !! ℓ = Some order1 →
+    own_all_preorders orders -∗
+    own_preorder_loc ℓ order2 -∗
+    ⌜ order1 = encode_relation order2 ⌝.
+  Proof.
+    iIntros (look) "auth frag".
+    iDestruct (own_valid_2 with "auth frag") as %[incl _]%auth_both_valid_discrete.
+    iPureIntro.
+    move: incl.
+    rewrite singleton_included_l.
+    intros [y [eq incl]].
+    move: incl.
+    rewrite lookup_fmap in eq.
+    rewrite look in eq.
+    apply equiv_Some_inv_r' in eq.
+    destruct eq as [y' [look' eq]].
+    rewrite eq.
+    rewrite <- look'.
+    rewrite Some_included_total.
+    rewrite to_agree_included.
+    intros eq'.
+    rewrite eq'.
+    done.
+  Qed.
+
+  (* If we know that two encoded values are related by en encoded relation, then
+  we can "recover" rela unencoded values taht are related by the unencoded
+  relation. *)
+  Lemma encode_relation_related (R : relation2 A) ea eb :
+    (encode_relation R) ea eb →
+    ∃ a b, decode ea = Some a ∧ decode eb = Some b ∧ R a b.
+  Proof.
+    rewrite /encode_relation.
+    destruct (decode ea) as [|a], (decode eb) as [|b]; try done.
+    intros ?. eexists _, _. done.
+  Qed.
+
+  Lemma encode_relation_decode_iff (R : relation2 A) ea eb (a b : A) :
+    decode ea = Some a →
+    decode eb = Some b →
+    (encode_relation R) ea eb →
+    R a b.
+  Proof. rewrite /encode_relation. intros -> ->. done. Qed.
+
+End preorders.
+
+Section points_to_shared.
+  Context `{!nvmG Σ}.
+
+  Implicit Types (Φ : val → dProp Σ) (e : expr).
+
+  Definition abs_hist_to_ra_old
+             (abs_hist : gmap time (message * positive)) : encoded_abs_historyR :=
+    (to_agree ∘ snd) <$> abs_hist.
+
+  Lemma singleton_included_l' `{Countable K} `{CmraTotal A} (m : gmap K A) (i : K) x :
+    {[i := x]} ≼ m ↔ (∃ y : A, m !! i ≡ Some y ∧ x ≼ y).
+  Proof.
+    setoid_rewrite <-(Some_included_total x).
+    apply singleton_included_l.
+  Qed.
+
+  Definition increasing_list `{AbstractState ST} (ss : list ST) :=
+    ∀ i j (s s' : ST), i ≤ j → (ss !! i = Some s) → (ss !! j = Some s') → s ⊑ s'.
+
+  (* _Exclusive_ points-to predicate. This predcate says that we know that the
+  last events at [ℓ] corresponds to the *)
+  Definition mapsto_ex `{AbstractState ST}
+             ℓ (ss1 ss2 : list ST)
+             (ϕ : ST → val → dProp Σ) : dProp Σ :=
+    (∃ (tGlobalPers tPers tStore : time) (abs_hist : abs_history ST),
+
+      "%incrList" ∷ ⌜ increasing_list (ss1 ++ ss2) ⌝ ∗
+      "#knowOrder" ∷ ⎡ own_preorder_loc ℓ ((⊑@{ST})) ⎤ ∗
+
+      "%lookupP" ∷ ⌜abs_hist !! tPers = head ss2⌝ ∗ (* Note: This also ensures that [ss2] is non-empty :) *)
+      (* [tStore] is the last message and it agrees with the last state in ss2. *)
+      "%lookupV" ∷ ⌜abs_hist !! tStore = last ss2⌝ ∗
+      "%nolater" ∷ ⌜(∀ t', tStore < t' → abs_hist !! t' = None)⌝ ∗
+
+      (* Ownership over the abstract history. *)
+      "hist" ∷ ⎡know_full_history_loc ℓ abs_hist⎤ ∗
+      (* Knowledge of the predicate. *)
+      "knowPred" ∷ ⎡know_pred ℓ ϕ⎤ ∗
+
+      "%slice" ∷ ⌜map_slice abs_hist tGlobalPers tStore (ss1 ++ ss2)⌝ ∗
+
+      (* We "have"/"know of" the three timestamps. *)
+      "%know" ∷ monPred_in ({[ ℓ := MaxNat tStore ]}, {[ ℓ := MaxNat tPers ]}, ∅) ∗
+      "per" ∷ ⎡persisted ({[ ℓ := MaxNat tGlobalPers ]} : view)⎤
+    ).
+
+  Global Instance mapsto_ex_discretizable `{AbstractState ST} ℓ ss1 ss2 ϕ :
+    Discretizable (mapsto_ex ℓ ss1 ss2 ϕ).
+  Proof. apply _. Qed.
+
+  (* This definition uses an existentially quantified [s']. We do this such that
+  owning [know_global_per_lower_bound ℓ s] before a crash also results in owning
+  exactly the same, [know_global_per_lower_bound ℓ s], after a crash. Had the
+  definition said that _exactly_ [s] was persisted at [t] then we would have a
+  different state after a crash, since after a crash there is only a single
+  entry in the history for [ℓ] and that entry may refer to any abstract state
+  greater than [s]. Said in another way, this definition allows for weakening
+  (lowering the state) which we do after a crash to get a simpler (but just as
+  useful) interaction with the post crash modality. *)
+  Definition know_global_per_lower_bound `{AbstractState ST} (ℓ : loc) (s : ST) : dProp Σ :=
+    ∃ t s', ⌜ s ⊑ s' ⌝ ∗
+            ⎡ own_preorder_loc ℓ abs_state_relation ∗
+              persisted {[ ℓ := MaxNat t ]} ∗
+              know_frag_history_loc ℓ {[ t := s' ]} ⎤.
+
+  Program Definition know_persist_lower_bound `{AbstractState ST} (ℓ : loc) (s : ST) : dProp Σ :=
+    MonPred (λ TV,
+      ∃ (t : nat) s',
+        ⌜ s ⊑ s' ⌝ ∗
+        ⌜t ≤ (persist_view TV) !!0 ℓ⌝ ∗
+        own_preorder_loc ℓ abs_state_relation ∗
+        know_frag_history_loc ℓ {[ t := s' ]}
+    )%I _.
+  Next Obligation. solve_proper. Qed.
+
+  Program Definition know_store_lower_bound `{AbstractState ST} (ℓ : loc) (s : ST) : dProp Σ :=
+    MonPred (λ TV,
+      ∃ (t : nat) s',
+        ⌜ s ⊑ s' ⌝ ∗
+        ⌜t ≤ (store_view TV) !!0 ℓ⌝ ∗
+        own_preorder_loc ℓ abs_state_relation ∗
+        know_frag_history_loc ℓ {[ t := s' ]}
+    )%I _.
+  Next Obligation. solve_proper. Qed.
+
+  Definition mapsto_shared `{AbstractState ST}
+             ℓ (s1 s2 s3 : ST) (ϕ : ST → val → dProp Σ) : dProp Σ :=
+    "knowPred" ∷ ⎡ know_pred ℓ ϕ ⎤ ∗
+    "isSharedLoc" ∷ ⎡ own shared_locs_name (◯ {[ ℓ ]}) ⎤ ∗
+    "globalPerLB" ∷ know_global_per_lower_bound ℓ s1 ∗
+    "persistLB" ∷ know_persist_lower_bound ℓ s2 ∗
+    "storeLB" ∷ know_store_lower_bound ℓ s3.
+
+  Global Instance know_persist_lower_bound_persistent `{AbstractState ST}
+         ℓ (s : ST) : Persistent (know_persist_lower_bound ℓ s).
+  Proof. apply monPred_persistent=> j. apply _. Qed.
+
+  Global Instance know_store_lower_bound_persistent `{AbstractState ST}
+         ℓ (s : ST) : Persistent (know_store_lower_bound ℓ s).
+  Proof. apply monPred_persistent=> j. apply _. Qed.
+
+  Lemma know_persist_lower_bound_at_zero `{AbstractState ST} ℓ (s s' : ST) :
+    s ⊑ s' →
+    ⎡ know_frag_history_loc ℓ {[0 := s']} ⎤ -∗
+    ⎡ own_preorder_loc ℓ abs_state_relation ⎤ -∗
+    know_persist_lower_bound ℓ s.
+  Proof.
+    iStartProof (iProp _). iIntros (incl ?) "?".
+    iIntros (? ?) "?". iExists 0, s'. iFrame "%∗". iPureIntro. lia.
+  Qed.
+
+  Lemma know_store_lower_bound_at_zero `{AbstractState ST} ℓ (s s' : ST) :
+    s ⊑ s' →
+    ⎡ know_frag_history_loc ℓ {[0 := s']} ⎤ -∗
+    ⎡ own_preorder_loc ℓ abs_state_relation ⎤ -∗
+    know_store_lower_bound ℓ s.
+  Proof.
+    iStartProof (iProp _). iIntros (incl ?) "?".
+    iIntros (? ?) "?". iExists 0, s'. iFrame "%∗". iPureIntro. lia.
+  Qed.
+
+End points_to_shared.
+
+(** Notation for the exclusive points-to predicate. *)
+Notation "l ↦ xs ; ys | P" := (mapsto_ex l xs ys P) (at level 20).
+
+(** Notation for the shared points-to predicate. *)
+Notation "l ↦ ( s1 , s2 , s3 )  | P" := (mapsto_shared l s1 s2 s3 P) (at level 20).
